lawyer/nonblocking/logrel/substitutions.v
@@ -1,0 +1,209 @@
+From fairness Require Import utils. 
+From heap_lang Require Import lang heap_lang_defs tactics. 
+
+Definition subst_env (vs: gmap string val) (e: expr) := 
+  map_fold subst e vs.
+
+Lemma subst_env_var x vs:
+  subst_env vs (Var x) = from_option Val (Var x) (vs !! x).
+Proof using.
+  rewrite /subst_env.
+  
+  set (P := fun (e: expr) (mp: gmap string val) =>
+              e = from_option Val (Var x) (mp !! x)).
+  enough (P (map_fold subst (Var x) vs) vs).
+  { done. }
+  
+  apply map_fold_weak_ind; clear vs. 
+  { done. }
+  subst P. simpl. intros s v vs e NIN ->.
+  rewrite insert_union_singleton_l. rewrite lookup_union.
+  rewrite lookup_map_singleton.
+  
+  destruct decide as [-> | NEQ]. 
+  { simpl. rewrite NIN. simpl. by rewrite decide_True. }
+  rewrite option_union_left_id.
+  destruct (vs !! x) eqn:XTH.
+  - simpl. done.
+  - simpl. by rewrite decide_False.
+Qed.
+
+(* TODO: move *)
+Lemma foldl_foldr_rev {A B : Type} (f : B → A → B) (b : B) (la : list A):
+  foldl f b la = foldr (flip f) b (rev la). 
+Proof using.
+  generalize dependent b. induction la.
+  { done. }
+  simpl. intros. rewrite IHla.
+  by rewrite foldr_app.
+Qed.
+
+Lemma subst_env_arg3
+  (F: expr -> expr -> expr -> expr)
+  (DISTR: forall e1 e2 e3 s v, subst s v (F e1 e2 e3) = F (subst s v e1) (subst s v e2) (subst s v e3)):
+  forall e1 e2 e3 vs, subst_env vs (F e1 e2 e3) = F (subst_env vs e1) (subst_env vs e2) (subst_env vs e3).
+Proof using.
+  intros. rewrite /subst_env.
+  pattern vs. apply map_first_key_ind. 
+  { intros. by rewrite !map_fold_empty. }
+  intros s v m NIN FKEY IH.
+  rewrite !map_fold_insert_first_key; auto.
+  by rewrite IH.
+Qed.
+
+Lemma subst_env_arg2 (F: expr -> expr -> expr)
+  (DISTR: forall e1 e2 s v, subst s v (F e1 e2) = F (subst s v e1) (subst s v e2)):
+  forall e1 e2 vs, subst_env vs (F e1 e2) = F (subst_env vs e1) (subst_env vs e2).
+Proof using.
+  intros. rewrite /subst_env.
+  pattern vs. apply map_first_key_ind. 
+  { intros. by rewrite !map_fold_empty. }
+  intros s v m NIN FKEY IH.
+  rewrite !map_fold_insert_first_key; auto.
+  by rewrite IH.
+Qed.
+
+Lemma subst_env_arg1 (F: expr -> expr)
+  (DISTR: forall e1 s v, subst s v (F e1) = F (subst s v e1)):
+  forall e1 vs, subst_env vs (F e1) = F (subst_env vs e1).
+Proof using.
+  intros. rewrite /subst_env.
+  pattern vs. apply map_first_key_ind. 
+  { intros. by rewrite !map_fold_empty. }
+  intros s v m NIN FKEY IH.
+  rewrite !map_fold_insert_first_key; auto.
+  by rewrite IH.
+Qed.
+
+Definition rm_binder (b: binder) (vs: gmap string val) :=
+  match b with 
+  | BNamed s => delete s vs
+  | BAnon => vs
+  end.
+
+Lemma subst_env_empty e: subst_env ∅ e = e.
+Proof using. done. Qed.
+
+Lemma subst_env_singleton s v e: subst_env {[ s := v ]} e = subst s v e.
+Proof using.
+  rewrite /subst_env. by rewrite map_fold_singleton.
+Qed.
+
+Lemma rm_binder_empty b: rm_binder b ∅ = ∅.
+Proof using. destruct b; set_solver. Qed.
+
+Ltac gd x := generalize dependent x. 
+
+Lemma subst_comm s1 v1 s2 v2 e
+  (NEQ: s1 ≠ s2):
+  subst s1 v1 (subst s2 v2 e) = subst s2 v2 (subst s1 v1 e).
+Proof using.
+  gd s1. gd v1. gd s2. gd v2. 
+  induction e; intros; simpl; try done.
+  all: try by (f_equal; eauto).
+  - destruct decide, decide; subst; simpl; try done.
+    + by rewrite decide_True.
+    + by rewrite decide_True.
+    + by rewrite !decide_False.
+  - destruct decide, decide; subst; simpl; try done.
+    f_equal. eauto.
+Qed.
+
+Lemma subst_env_insert s v vs e
+  (FRESH: s ∉ dom vs):
+  subst_env (<[ s := v ]> vs) e = subst s v (subst_env vs e).
+Proof using.
+  rewrite /subst_env.
+  eapply map_fold_insert_L.
+  2: by apply not_elem_of_dom.
+  intros. by apply subst_comm.
+Qed.
+
+Lemma subst_env_insert' s v vs e
+  (FRESH: s ∉ dom vs):
+  subst_env (<[ s := v ]> vs) e = subst_env vs (subst s v e). 
+Proof using.
+  rewrite subst_env_insert; [| done].
+  (* TODO: extract lemma *)
+  gd e. revert FRESH. pattern vs. apply map_first_key_ind; clear vs. 
+  { intros. by rewrite !subst_env_empty. }
+  intros. rewrite subst_env_insert; [| by apply not_elem_of_dom].
+  rewrite dom_insert_L in FRESH. 
+  apply not_elem_of_union in FRESH as [?%not_elem_of_singleton ?].
+  rewrite subst_comm; [| done].
+  rewrite H1; [| done].  
+  rewrite -subst_env_insert; [| by apply not_elem_of_dom]. 
+  done.
+Qed.
+
+Lemma rm_binder_insert_comm b s v vs
+  (NEQ: b ≠ BNamed s):
+  rm_binder b (<[ s := v ]> vs) = <[ s := v ]> (rm_binder b vs).
+Proof using.
+  destruct b as [| sb]; simpl. 
+  { done. }
+  apply map_eq. intros s'.
+  Set Printing Coercions.
+  assert (sb ≠ s).
+  { congruence. }
+  destruct (decide (s' = s)) as [-> | NEQ'].
+  { rewrite lookup_delete_ne; [| done].
+    by rewrite !lookup_insert. }
+  rewrite lookup_insert_ne; [| done].
+  destruct (decide (sb = s')) as [-> | NEQ''].
+  { by rewrite !lookup_delete. }
+  do 2 (rewrite lookup_delete_ne; [| done]).
+  rewrite lookup_insert_ne; done.
+Qed.
+
+Lemma dom_rm_binder b vs:
+  dom (rm_binder b vs) = dom vs ∖ match b with | BNamed s => {[ s ]} | _ => ∅ end.
+Proof using.
+  rewrite /rm_binder. destruct b; set_solver.
+Qed.
+
+Lemma rm_binder_subseteq s vs:
+  rm_binder s vs ⊆ vs.
+Proof using.
+  destruct s; simpl; try set_solver.
+  apply delete_subseteq.
+Qed. 
+    
+Lemma subst_env_rec (b x: binder) (f: expr) vs:
+  let vs' := rm_binder b $ rm_binder x vs in
+  subst_env vs (Rec b x f) = Rec b x (subst_env vs' f).
+Proof using.
+  simpl. generalize dependent f. 
+  pattern vs. apply map_first_key_ind; clear vs. 
+  { intros. by rewrite !rm_binder_empty !subst_env_empty. }
+  intros s v vs NIN FKEY IH f.
+  rewrite subst_env_insert; [| by apply not_elem_of_dom].
+  rewrite IH. simpl. f_equal.
+  destruct decide.
+  - destruct a. 
+    rewrite -subst_env_insert.
+    2: { rewrite !dom_rm_binder.
+         apply not_elem_of_dom in NIN.
+         destruct x, b; set_solver. }
+    rewrite rm_binder_insert_comm; [| done].
+    f_equal. rewrite rm_binder_insert_comm; [| done].
+    done. 
+  - apply Classical_Prop.not_and_or in n.
+    destruct (decide (BNamed s = x)) as [<- | ?]; simpl. 
+    + by rewrite delete_insert_delete.
+    + rewrite rm_binder_insert_comm; [| done].
+      destruct n as [<-%NNP_P | <-%NNP_P]; simpl; try done.
+      by rewrite delete_insert_delete.
+Qed.
+
+Lemma subst_subst_ignored s v v' e:
+  subst s v' (subst s v e) = subst s v e.
+Proof using.
+  gd v. gd v'. induction e; simpl; try done.
+  all: try by (intros; f_equal; eauto).
+  - intros. destruct decide; try done. simpl.
+    by rewrite decide_False.
+  - destruct decide; try done.
+    intros. f_equal. eauto.
+Qed.
+
